adhoc (and not safe) support for the opcode GAS

ver2/stack_operation_instructions.v
@@ -468,6 +468,13 @@ let address := get_address_ctx ctx in
 Definition evm_basefee (ctx : context) (args : list EVMWord) : EVMWord :=
 get_basefee_ctx ctx.
 
+Definition evm_gas (ctx : context) (args : list EVMWord) : EVMWord :=
+  WZero.
+Lemma gas_ctx_ind: ctx_independent_op evm_gas.
+Proof.
+  ctx_independent_tac evm_gas.
+Qed.
+
 
 Definition evm_stack_opm : stack_op_instr_map :=
   ADD |->i OpImp 2 evm_add (Some add_comm) (Some add_ctx_ind);
@@ -515,7 +522,8 @@ Definition evm_stack_opm : stack_op_instr_map :=
   GASLIMIT |->i OpImp 0 evm_gaslimit None None;
   CHAINID |->i OpImp 0 evm_chainid None None;
   SELFBALANCE |->i OpImp 0  evm_selfbalance None None;
-  BASEFEE |->i OpImp 0 evm_basefee None None.
+  BASEFEE |->i OpImp 0 evm_basefee None None;
+  GAS |->i OpImp 0 evm_gas None (Some gas_ctx_ind).
  
 
 
